\documentclass[11pt]{article}

\usepackage[top=1in,right=1in,left=1in,bottom=1in]{geometry}

\usepackage{amssymb}
\usepackage{amsmath}

\begin{document}

\begin{flushright}
  Kyle Cesare
\end{flushright}

{\center \textbf{Math Write-up 5} \\}

Given a function $F(x, y, z(x, y)) = 0$ that implicitly defines $z$ as a
differentiable function of $x$ and $y$, prove that

$$
  \frac{ \partial z }{ \partial x } = -\frac{ F_x }{ F_z } \text{ and }
  \frac{ \partial z }{ \partial y } = -\frac{ F_y }{ F_z }
$$

We know that, as $F(x, y, z(x, y)) = 0$ and $z$ is implicitly defined as a
function of $x$ and $y$, we can say that

$$
  z(x, y) = -F(x, y)
$$

We can use the chain rule to solve for the partial derivatives we want

\begin{align*}
  \frac{ \partial z }{ \partial x } \frac{ dz }{ dx }
    &= -\frac{ \partial F }{ \partial x } \frac{ \partial x }{ \partial z } \\
  \frac{ dz }{ dx } 
    &= -\frac{ \partial F }{ \partial z } / \frac{ \partial F }{ \partial x } \\
    &= -\frac{ F_x }{ F_z } \\
  \frac{ \partial z }{ \partial y } \frac{ dz }{ dy }
    &= -\frac{ \partial F }{ \partial y } \frac{ \partial y }{ \partial z } \\
  \frac{ dz }{ dy } 
    &= -\frac{ \partial F }{ \partial z } / \frac{ \partial F }{ \partial y } \\
    &= -\frac{ F_y }{ F_z }
\end{align*}

Now we can solve for $F_x$ and $F_y$ in $xy + xz + yz = 3$

\begin{align*}
  \frac{ \partial z }{ \partial x }
    &= -\frac{ F_x }{ F_z } \\
    &= -\frac{ y + z }{ x + y } \\
  \frac{ \partial z }{ \partial y }
    &= -\frac{ F_y }{ F_z } \\
    &= -\frac{ x + z }{ x + y } \\
\end{align*}

\end{document}
